began semantic preservation theorem

src/ewacket.v
@@ -1,15 +1,42 @@
 Require Import Arith Bool List ZArith.
+Local Open Scope Z_scope.
+
 Require Import wacket.
-Require Import observable.
+Require Import wasmLite.
 Require Import compiler.
 
 
 
 
+Definition dupeResult_to_wasmVal (res: dupeResult) :=
+match res with 
+| DR_Int z => v_i64 z
+| DR_Bool b => if b then v_i32 1 else v_i32 0
+| DR_Error => trap
+end.
 
+(* going to need that dupe is well typed, 
+and therefor evalDupe cannot produce an error, 
+honestly this should be a feature of the compiler*)
 Theorem semanticPreservation:
-    forall (S : dupe) (C : wasm) (obs: observable), (wasmCompiler S) = (Succ C) ->
-    (S d==> obs) -> (C c==> obs).
+    forall source compiled result,
+    (compile_unsafe source) = compiled ->
+    (dupeResult_to_wasmVal (evalDupe source)) = result ->
+    (compiled,nil) w-->* ((nil, result::nil)).
 Proof.
+    induction source; intros;
+    (try (
+        rewrite <- H;rewrite <- H0;
+        (try destruct b);
+        econstructor;constructor; reflexivity
+    )).
+    - simpl in H. 
+        rewrite <- (app_nil_l compiled) in H. 
+        apply app_eq_app in H. 
+        do 3 destruct H.
+        + rewrite app_nil_l in H.
+            simpl in H0.
+
+    
 Admitted.
 
